theories/L/Functions/Encoding.v
@@ -3,25 +3,35 @@ From Undecidability.L.Datatypes Require Export LNat LTerm LProd.
 
 (** ** Extracted encoding of natural numbers *)
 
-Instance term_nat_enc : computableTime' nat_enc (fun n _ => (n * 14 + 12,tt)).
+Instance term_nat_enc : computableTime' (enc (X:=nat)) (fun n _ => (n * 14 + 12,tt)).
 Proof.
+  unfold enc. cbn.
   extract. solverec.
 Qed.
 
 (** ** Extracted term encoding *)
 
-Instance term_term_enc : computableTime' term_enc (fun s _ => (size s * 30,tt)).
+Instance term_term_enc : computableTime' (enc (X:=term)) (fun s _ => (size s * 30,tt)).
 Proof.
+  unfold enc;cbn.
   extract. solverec.
 Qed.
 
-(* (** ** Extracted tuple encoding *) *)
+(** ** Extracted tuple encoding *)
 
-(* Instance term_prod_enc X Y (R1:registered X) (R2:registered Y): computable (@prod_enc X Y R1 R2). *)
-(* Proof. *)
-(*   unfold prod_enc. cbn. extract. *)
-(* Qed. *)
+Instance term_prod_enc X Y (R1:registered X) (R2:registered Y) t__X t__Y
+         `{computableTime' (@enc X _) t__X} `{computableTime' (@enc Y _) t__Y}
+  :computableTime' (@prod_enc X Y R1 R2) (fun w _ => (let '(x,y):= w in  fst (t__X x tt) + fst (t__Y y tt) + 15,tt)).
+Proof.
+  unfold prod_enc. fold (@enc X _). fold (@enc Y _).
+  extract. solverec.
+Qed.
 
+(*
+Set Printing Implicit.
+Check (extT (@enc (nat*(nat*nat)) _)).
+*)
+(*
 Definition prod_enc' {X Y} (enc_x : X -> term) (enc_y : Y -> term) : X * Y -> term :=
   fix f w := let '(x,y) := w in
              lam (var 0 (enc_x x) (enc_y y)).
@@ -37,3 +47,4 @@ Instance term_prod_enc' {X Y} {H__x : registered X} {H__Y : registered Y}:
 Proof.
   extract. solverec.
 Qed.
+*)
